simplify. Make more inline with spec FIPS 180-4

examples/sha256/proofs/fstar/spec/Sha256.fst
@@ -1,34 +1,30 @@
 module Sha256
 
-#set-options "--max_fuel 25 --max_ifuel 25 --z3rlimit 60 --query_stats"
-
 open Core
+
+open FStar.Mul
 
 open FStar.Seq
 
-
 let v_BLOCK_SIZE:usize = mk_usize 64
+
 let v_LEN_SIZE:usize = mk_usize 8
+
 let v_K_SIZE:usize = mk_usize 64
+
 let v_HASH_SIZE:usize = mk_usize (256 / 8)
 
 type t_Block = t_Array u8 v_BLOCK_SIZE
+
 type t_OpTableType = t_Array u8 (mk_usize 12)
+
 type t_Sha256Digest = t_Array u8 v_HASH_SIZE
+
 type t_RoundConstantsTable = t_Array u32 v_K_SIZE
+
 type t_Hash = t_Array u32 v_LEN_SIZE
 
-let v_OP_TABLE: t_OpTableType =
-  let list =
-    [
-      mk_u8 2; mk_u8 13; mk_u8 22; mk_u8 6; mk_u8 11; mk_u8 25; mk_u8 7; mk_u8 18; mk_u8 3; mk_u8 17;
-      mk_u8 19; mk_u8 10
-    ]
-  in
-  FStar.Pervasives.assert_norm (Prims.eq2 (List.Tot.length list) 12);
-  Rust_primitives.Hax.array_of_list 12 list
-
-let v_K_TABLE: t_RoundConstantsTable =
+let v_K_TABLE:t_RoundConstantsTable =
   let list =
     [
       mk_u32 1116352408; mk_u32 1899447441; mk_u32 3049323471; mk_u32 3921009573; mk_u32 961987163;
@@ -49,7 +45,7 @@ let v_K_TABLE: t_RoundConstantsTable =
   FStar.Pervasives.assert_norm (Prims.eq2 (List.Tot.length list) 64);
   Rust_primitives.Hax.array_of_list 64 list
 
-let v_HASH_INIT: t_Hash =
+let v_HASH_INIT:t_Hash =
   let list =
     [
       mk_u32 1779033703;
@@ -65,171 +61,113 @@ let v_HASH_INIT: t_Hash =
   FStar.Pervasives.assert_norm (Prims.eq2 (List.Tot.length list) 8);
   Rust_primitives.Hax.array_of_list 8 list
 
-let ch (x y z: u32) : u32 = (x &. y) ^. (~.x &. z)
 
-let maj (x y z: u32) : u32 = (x &. y) ^. (x &. z) ^. (y &. z)
 
-let sigma (x: u32) (i: usize{i <. mk_usize 4}) (op: usize) : u32 =
-  let tmp:u32 =
-    x >>>.
-    Core.Convert.f_into #u8
-      #u32
-      #FStar.Tactics.Typeclasses.solve
-      (v_OP_TABLE.[ (mk_usize 3) *! i +! (mk_usize 2) ] <: u8)
-  in
-  let tmp:u32 =
-    if op =. mk_usize 0 then x >>! (v_OP_TABLE.[ (mk_usize 3) *! i +! (mk_usize 2) ] <: u8) else tmp
-  in
-  let rot_val_1:u32 =
-    Core.Convert.f_into #u8 #u32 #FStar.Tactics.Typeclasses.solve v_OP_TABLE.[ (mk_usize 3) *! i ]
-  in
-  let rot_val_2:u32 =
-    Core.Convert.f_into #u8
-      #u32
-      #FStar.Tactics.Typeclasses.solve
-      v_OP_TABLE.[ (mk_usize 3) *! i +! (mk_usize 1) ]
-  in
-  // TODO: Figure out why <: u32 is needed here twice
-  (x >>>. rot_val_1 <: u32) ^. (x >>>. rot_val_2 <: u32) ^. tmp
+// FIPS PUB 180-4, Section 4.1.2
 
-let to_be_u32s (block: t_Block) : Alloc.Vec.t_Vec u32 Alloc.Alloc.t_Global =
-  let out:Alloc.Vec.t_Vec u32 Alloc.Alloc.t_Global =
-    Alloc.Vec.impl__with_capacity #u32 (v_BLOCK_SIZE /! mk_usize 4)
-  in
-  let out:Alloc.Vec.t_Vec u32 Alloc.Alloc.t_Global =
-    Core.Iter.Traits.Iterator.f_fold (Core.Iter.Traits.Collect.f_into_iter (Core.Slice.impl__chunks_exact
-              #u8
-              block
-              (mk_usize 4)))
-      out
-      (fun out block_chunk ->
-          let out:Alloc.Vec.t_Vec u32 Alloc.Alloc.t_Global = out in
-          let block_chunk_array =
-            Core.Num.impl_u32__from_be_bytes (Core.Result.impl__unwrap #(t_Array u8 (mk_usize 4))
-                  (Core.Convert.f_try_into #(t_Slice u8) #(t_Array u8 (mk_usize 4)) block_chunk))
-          in
-          let out:Alloc.Vec.t_Vec u32 Alloc.Alloc.t_Global =
-            Alloc.Vec.impl_1__push #u32 #Alloc.Alloc.t_Global out block_chunk_array
-          in
-          out)
-  in
-  out
+let f_ch (x y z: u32) : u32 = (x &. y) ^. (~.x &. z)
 
-let schedule (block: t_Block) : t_RoundConstantsTable =
-  let b = to_be_u32s block in
-  let s: t_RoundConstantsTable = Rust_primitives.Hax.repeat (mk_u32 0) (mk_usize 64) in
-  let s: t_RoundConstantsTable =
-    Rust_primitives.Hax.Folds.fold_range (mk_usize 0)
-      (mk_usize 16)
-      (fun _ _ -> true)
-      s
-      (fun s (i: usize) ->
-          let s: t_RoundConstantsTable = s in
-          if i <. mk_usize 16 <: b bool
-          then
-            let s: t_RoundConstantsTable =
-              Rust_primitives.Hax.Monomorphized_update_at.update_at_usize s i b.[ i ]
-            in
-            s
-          else
-            let t16:u32 = s.[ i -! mk_usize 16 ] in
-            let t15:u32 = s.[ i -! mk_usize 15 ] in
-            let t7:u32 = s.[ i -! mk_usize 7 ] in
-            let t2:u32 = s.[ i -! mk_usize 2 ] in
-            let s1:u32 = sigma t2 (mk_usize 3) (mk_usize 0) in
-            let s0:u32 = sigma t15 (mk_usize 2) (mk_usize 0) in
-            let s: t_RoundConstantsTable =
-              Rust_primitives.Hax.Monomorphized_update_at.update_at_usize s
-                i
-                (s1 +. t7 +. s0 +. t16)
-            in
-            s)
-  in
-  s
+let f_maj (x y z: u32) : u32 = (x &. y) ^. (x &. z) ^. (y &. z)
 
-let shuffle (ws: t_RoundConstantsTable) (hashi: t_Hash) : t_Hash =
-  let h: t_Hash = hashi in
-  let h: t_Hash =
-    Rust_primitives.Hax.Folds.fold_range (mk_usize 0)
-      v_K_SIZE
-      (fun _ _ -> true)
-      h
-      (fun (h: t_Array u32 (mk_usize 8)) i ->
-          let a0:u32 = h.[ mk_usize 0 ] in
-          let b0:u32 = h.[ mk_usize 1 ] in
-          let c0:u32 = h.[ mk_usize 2 ] in
-          let d0:u32 = h.[ mk_usize 3 ] in
-          let e0:u32 = h.[ mk_usize 4 ] in
-          let f0:u32 = h.[ mk_usize 5 ] in
-          let g0:u32 = h.[ mk_usize 6 ] in
-          let h0:u32 = h.[ mk_usize 7 ] in
-          let t1:u32 =
-            h0 +. (sigma e0 (mk_usize 1) (mk_usize 1)) +. (ch e0 f0 g0) +. v_K_TABLE.[ i ]
-          in
-          let t2:u32 = (sigma a0 (mk_usize 0) (mk_usize 1)) +. (maj a0 b0 c0) in
-          let h:t_Array u32 (mk_usize 8) =
-            Rust_primitives.Hax.Monomorphized_update_at.update_at_usize h (mk_usize 0) (t1 +. t2)
-          in
-          let h:t_Array u32 (mk_usize 8) =
-            Rust_primitives.Hax.Monomorphized_update_at.update_at_usize h (mk_usize 1) a0
-          in
-          let h:t_Array u32 (mk_usize 8) =
-            Rust_primitives.Hax.Monomorphized_update_at.update_at_usize h (mk_usize 2) b0
-          in
-          let h:t_Array u32 (mk_usize 8) =
-            Rust_primitives.Hax.Monomorphized_update_at.update_at_usize h (mk_usize 3) c0
-          in
-          let h:t_Array u32 (mk_usize 8) =
-            Rust_primitives.Hax.Monomorphized_update_at.update_at_usize h (mk_usize 4) (d0 +. t1)
-          in
-          let h:t_Array u32 (mk_usize 8) =
-            Rust_primitives.Hax.Monomorphized_update_at.update_at_usize h (mk_usize 5) e0
-          in
-          let h:t_Array u32 (mk_usize 8) =
-            Rust_primitives.Hax.Monomorphized_update_at.update_at_usize h (mk_usize 6) f0
-          in
-          let h:t_Array u32 (mk_usize 8) =
-            Rust_primitives.Hax.Monomorphized_update_at.update_at_usize h (mk_usize 7) g0
-          in
-          h)
-  in
-  h
+let f_SIGMA_0 x : u32 = (x >>>. mk_u32 2) ^. (x >>>. mk_u32 13) ^. (x >>>. mk_u32 22)
 
-let compress (block: t_Block) (h_in: t_Hash) : t_Hash =
-  let s: t_RoundConstantsTable = schedule block in
-  let h: t_Hash = shuffle s h_in in
-  let h: t_Hash =
-    Rust_primitives.Hax.Folds.fold_range (mk_usize 0)
-      (mk_usize 8)
-      (fun _ _ -> true)
-      h
-      (fun (h: t_Array u32 (mk_usize 8)) i ->
-          Rust_primitives.Hax.Monomorphized_update_at.update_at_usize h i (h.[ i ] +. h_in.[ i ]))
-  in
-  h
+let f_SIGMA_1 x : u32 = (x >>>. mk_u32 6) ^. (x >>>. mk_u32 11) ^. (x >>>. mk_u32 25)
 
-let u32s_to_be_bytes (state: t_Hash) : t_Sha256Digest =
-  let out: t_Sha256Digest = Rust_primitives.Hax.repeat (mk_u8 0) v_HASH_SIZE in
-  let out: t_Sha256Digest =
-    Rust_primitives.Hax.Folds.fold_range (mk_usize 0)
-      v_LEN_SIZE
-      (fun _ _ -> true)
-      out
-      (fun (out: t_Sha256Digest) i ->
-          let tmp:u32 = state.[ i ] in
-          let tmp:t_Array u8 (mk_usize 4) = Core.Num.impl_u32__to_be_bytes tmp in
-          Rust_primitives.Hax.Folds.fold_range (mk_usize 0)
-            (mk_usize 4)
-            (fun _ _ -> true)
-            out
-            (fun (out: t_Sha256Digest) j ->
-                Rust_primitives.Hax.Monomorphized_update_at.update_at_usize out
-                  ((i *! mk_usize 4) +! j)
-                  (tmp.[ j ])))
-  in
-  out
-  
+let f_sigma_0 x : u32 = (x >>>. mk_u32 7) ^. (x >>>. mk_u32 18) ^. (x >>! mk_u32 3)
+
+let f_sigma_1 x : u32 = (x >>>. mk_u32 17) ^. (x >>>. mk_u32 19) ^. (x >>! mk_u32 10)
+
+
+
+// FIPS PUB 180-4, Section 5.2.1
+
+let f_parse_message_block (block: t_Block) : t_Array u32 (mk_usize 16) =
+  createi (mk_usize 16)
+    (fun i ->
+        Core.Num.impl_u32__from_be_bytes (createi (mk_usize 4)
+              (fun j -> Seq.index block (4 * v i + v j))))
+
+
+
+// FIBS PUB 180-4, Section 6.2.2, Step 1
+
+let rec f_schedule_word (block: t_Block) (t: nat{t < 64}) : Tot u32 (decreases t) =
+  if t < 16
+  then
+    let b = f_parse_message_block block in
+    Seq.index b t
+  else
+    let w16 = f_schedule_word block (t - 16) in
+    let w15 = f_schedule_word block (t - 15) in
+    let w7 = f_schedule_word block (t - 7) in
+    let w2 = f_schedule_word block (t - 2) in
+    let s1 = f_sigma_1 w2 in
+    let s0 = f_sigma_0 w15 in
+    s1 +. w7 +. s0 +. w16
+
+let f_schedule (block: t_Block) : t_RoundConstantsTable =
+  createi (mk_usize 64) (fun i -> f_schedule_word block (v i))
+
+
+
+// FIPS PUB 180-4, Section 6.2.2, Step 2, 3 and 4
+
+let f_shuffle (ws: t_RoundConstantsTable) (hashi: t_Hash) : t_Hash =
+  Rust_primitives.Hax.Folds.fold_range (mk_usize 0)
+    v_K_SIZE
+    (fun _ _ -> true)
+    hashi
+    (fun (hash: t_Hash) (i: usize{i <. v_K_SIZE}) ->
+        let a = Seq.index hash 0 in
+        let b = Seq.index hash 1 in
+        let c = Seq.index hash 2 in
+        let d = Seq.index hash 3 in
+        let e = Seq.index hash 4 in
+        let f = Seq.index hash 5 in
+        let g = Seq.index hash 6 in
+        let h = Seq.index hash 7 in
+        let t1 = h +. (f_SIGMA_1 e) +. (f_ch e f g) +. v_K_TABLE.[ i ] +. ws.[ i ] in
+        let t2 = (f_SIGMA_0 a) +. (f_maj a b c) in
+        let hash = Seq.upd hash 0 (t1 +. t2) in
+        let hash = Seq.upd hash 1 a in
+        let hash = Seq.upd hash 2 b in
+        let hash = Seq.upd hash 3 c in
+        let hash = Seq.upd hash 4 (d +. t1) in
+        let hash = Seq.upd hash 5 e in
+        let hash = Seq.upd hash 6 f in
+        let hash = Seq.upd hash 7 g in
+        hash)
+
+
+
+// FIPS PUB 180-4, Section 6.2.2, Iterations
+
+let f_compress (block: t_Block) (h_in: t_Hash) : t_Hash =
+  let s = f_schedule block in
+  let h = f_shuffle s h_in in
+  Rust_primitives.Hax.Folds.fold_range (mk_usize 0)
+    v_LEN_SIZE
+    (fun _ _ -> true)
+    h
+    (fun (h: t_Hash) i -> Seq.upd h (v i) (h.[ i ] +. h_in.[ i ]))
+
+
+
+// FIPS PUB 180-4, Section 6.2.2, Last Step
+
+let f_hash_to_digest (hash: t_Hash) : t_Sha256Digest =
+  createi v_HASH_SIZE
+    (fun i ->
+        let word_index = v i / 4 in
+        let byte_index = v i % 4 in
+        let word = hash.[ mk_usize word_index ] in
+        let word_bytes = Core.Num.impl_u32__to_be_bytes word in
+        word_bytes.[ mk_usize byte_index ])
+
+
+
 // TOOD
-let hash (msg: t_Slice u8) : t_Sha256Digest = admit()
 
-let sha256 (msg: t_Slice u8) : t_Array u8 (mk_usize 32) = hash msg
+let hash (msg: t_Slice u8) : t_Sha256Digest = admit ()
+
+let sha256 msg = hash msg
